HelloWorld.thy
@@ -1,18 +1,18 @@
 theory HelloWorld
-  imports IO_Monad
+  imports IO
 begin
 
 section\<open>Hello, World!\<close>
 
 text\<open>
-  The idea of a \<^term>\<open>main :: unit IO\<close> function is that, upon start of your program, you will be
+  The idea of a \<^term>\<open>main :: unit io\<close> function is that, upon start of your program, you will be
   handed a value of type \<^typ>\<open>real_world\<close>. You can pass this world through your code and modify it.
   Be careful with the \<^typ>\<open>real_world\<close>, it's the only one we have.
 \<close>
 
 
 text\<open>The main function, defined in Isabelle. It should have the right type in Haskell.\<close>
-definition main :: "unit IO" where
+definition main :: "unit io" where
   "main \<equiv> do {
                _ \<leftarrow> println (STR ''Hello World! What is your name?'');
                name \<leftarrow> getLine;
